Elimination of the archaic ASCII syntax

src/HOL/Auth/OtwayRees_AN.thy
@@ -28,31 +28,31 @@ inductive_set otway :: "event list set"
 
  | Fake: \<comment> \<open>The Spy may say anything he can say.  The sender field is correct,
             but agents don't use that information.\<close>
-         "[| evsf \<in> otway;  X \<in> synth (analz (knows Spy evsf)) |]
-          ==> Says Spy B X  # evsf \<in> otway"
+         "\<lbrakk>evsf \<in> otway;  X \<in> synth (analz (knows Spy evsf))\<rbrakk>
+          \<Longrightarrow> Says Spy B X  # evsf \<in> otway"
 
         
  | Reception: \<comment> \<open>A message that has been sent can be received by the
                   intended recipient.\<close>
-              "[| evsr \<in> otway;  Says A B X \<in>set evsr |]
-               ==> Gets B X # evsr \<in> otway"
+              "\<lbrakk>evsr \<in> otway;  Says A B X \<in>set evsr\<rbrakk>
+               \<Longrightarrow> Gets B X # evsr \<in> otway"
 
  | OR1:  \<comment> \<open>Alice initiates a protocol run\<close>
          "evs1 \<in> otway
-          ==> Says A B \<lbrace>Agent A, Agent B, Nonce NA\<rbrace> # evs1 \<in> otway"
+          \<Longrightarrow> Says A B \<lbrace>Agent A, Agent B, Nonce NA\<rbrace> # evs1 \<in> otway"
 
  | OR2:  \<comment> \<open>Bob's response to Alice's message.\<close>
-         "[| evs2 \<in> otway;
-             Gets B \<lbrace>Agent A, Agent B, Nonce NA\<rbrace> \<in>set evs2 |]
-          ==> Says B Server \<lbrace>Agent A, Agent B, Nonce NA, Nonce NB\<rbrace>
+         "\<lbrakk>evs2 \<in> otway;
+             Gets B \<lbrace>Agent A, Agent B, Nonce NA\<rbrace> \<in>set evs2\<rbrakk>
+          \<Longrightarrow> Says B Server \<lbrace>Agent A, Agent B, Nonce NA, Nonce NB\<rbrace>
                  # evs2 \<in> otway"
 
  | OR3:  \<comment> \<open>The Server receives Bob's message.  Then he sends a new
            session key to Bob with a packet for forwarding to Alice.\<close>
-         "[| evs3 \<in> otway;  Key KAB \<notin> used evs3;
+         "\<lbrakk>evs3 \<in> otway;  Key KAB \<notin> used evs3;
              Gets Server \<lbrace>Agent A, Agent B, Nonce NA, Nonce NB\<rbrace>
-               \<in>set evs3 |]
-          ==> Says Server B
+               \<in>set evs3\<rbrakk>
+          \<Longrightarrow> Says Server B
                \<lbrace>Crypt (shrK A) \<lbrace>Nonce NA, Agent A, Agent B, Key KAB\<rbrace>,
                  Crypt (shrK B) \<lbrace>Nonce NB, Agent A, Agent B, Key KAB\<rbrace>\<rbrace>
               # evs3 \<in> otway"
@@ -60,20 +60,20 @@ inductive_set otway :: "event list set"
  | OR4:  \<comment> \<open>Bob receives the Server's (?) message and compares the Nonces with
              those in the message he previously sent the Server.
              Need \<^term>\<open>B \<noteq> Server\<close> because we allow messages to self.\<close>
-         "[| evs4 \<in> otway;  B \<noteq> Server;
+         "\<lbrakk>evs4 \<in> otway;  B \<noteq> Server;
              Says B Server \<lbrace>Agent A, Agent B, Nonce NA, Nonce NB\<rbrace> \<in>set evs4;
              Gets B \<lbrace>X, Crypt(shrK B)\<lbrace>Nonce NB,Agent A,Agent B,Key K\<rbrace>\<rbrace>
-               \<in>set evs4 |]
-          ==> Says B A X # evs4 \<in> otway"
+               \<in>set evs4\<rbrakk>
+          \<Longrightarrow> Says B A X # evs4 \<in> otway"
 
  | Oops: \<comment> \<open>This message models possible leaks of session keys.  The nonces
              identify the protocol run.\<close>
-         "[| evso \<in> otway;
+         "\<lbrakk>evso \<in> otway;
              Says Server B
                       \<lbrace>Crypt (shrK A) \<lbrace>Nonce NA, Agent A, Agent B, Key K\<rbrace>,
                         Crypt (shrK B) \<lbrace>Nonce NB, Agent A, Agent B, Key K\<rbrace>\<rbrace>
-               \<in>set evso |]
-          ==> Notes Spy \<lbrace>Nonce NA, Nonce NB, Key K\<rbrace> # evso \<in> otway"
+               \<in>set evso\<rbrakk>
+          \<Longrightarrow> Notes Spy \<lbrace>Nonce NA, Nonce NB, Key K\<rbrace> # evso \<in> otway"
 
 
 declare Says_imp_knows_Spy [THEN analz.Inj, dest]
@@ -83,8 +83,8 @@ declare Fake_parts_insert_in_Un  [dest]
 
 
 text\<open>A "possibility property": there are traces that reach the end\<close>
-lemma "[| B \<noteq> Server; Key K \<notin> used [] |]
-      ==> \<exists>evs \<in> otway.
+lemma "\<lbrakk>B \<noteq> Server; Key K \<notin> used []\<rbrakk>
+      \<Longrightarrow> \<exists>evs \<in> otway.
            Says B A (Crypt (shrK A) \<lbrace>Nonce NA, Agent A, Agent B, Key K\<rbrace>)
              \<in> set evs"
 apply (intro exI bexI)
@@ -96,7 +96,7 @@ apply (possibility, simp add: used_Cons)
 done
 
 lemma Gets_imp_Says [dest!]:
-     "[| Gets B X \<in> set evs; evs \<in> otway |] ==> \<exists>A. Says A B X \<in> set evs"
+     "\<lbrakk>Gets B X \<in> set evs; evs \<in> otway\<rbrakk> \<Longrightarrow> \<exists>A. Says A B X \<in> set evs"
 by (erule rev_mp, erule otway.induct, auto)
 
 
@@ -104,8 +104,8 @@ by (erule rev_mp, erule otway.induct, auto)
 text\<open>For reasoning about the encrypted portion of messages\<close>
 
 lemma OR4_analz_knows_Spy:
-     "[| Gets B \<lbrace>X, Crypt(shrK B) X'\<rbrace> \<in> set evs;  evs \<in> otway |]
-      ==> X \<in> analz (knows Spy evs)"
+     "\<lbrakk>Gets B \<lbrace>X, Crypt(shrK B) X'\<rbrace> \<in> set evs;  evs \<in> otway\<rbrakk>
+      \<Longrightarrow> X \<in> analz (knows Spy evs)"
 by blast
 
 
@@ -114,15 +114,15 @@ NOBODY sends messages containing X!\<close>
 
 text\<open>Spy never sees a good agent's shared key!\<close>
 lemma Spy_see_shrK [simp]:
-     "evs \<in> otway ==> (Key (shrK A) \<in> parts (knows Spy evs)) = (A \<in> bad)"
+     "evs \<in> otway \<Longrightarrow> (Key (shrK A) \<in> parts (knows Spy evs)) = (A \<in> bad)"
 by (erule otway.induct, simp_all, blast+)
 
 lemma Spy_analz_shrK [simp]:
-     "evs \<in> otway ==> (Key (shrK A) \<in> analz (knows Spy evs)) = (A \<in> bad)"
+     "evs \<in> otway \<Longrightarrow> (Key (shrK A) \<in> analz (knows Spy evs)) = (A \<in> bad)"
 by auto
 
 lemma Spy_see_shrK_D [dest!]:
-     "[|Key (shrK A) \<in> parts (knows Spy evs);  evs \<in> otway|] ==> A \<in> bad"
+     "\<lbrakk>Key (shrK A) \<in> parts (knows Spy evs);  evs \<in> otway\<rbrakk> \<Longrightarrow> A \<in> bad"
 by (blast dest: Spy_see_shrK)
 
 
@@ -130,12 +130,12 @@ subsection\<open>Proofs involving analz\<close>
 
 text\<open>Describes the form of K and NA when the Server sends this message.\<close>
 lemma Says_Server_message_form:
-     "[| Says Server B
+     "\<lbrakk>Says Server B
             \<lbrace>Crypt (shrK A) \<lbrace>NA, Agent A, Agent B, Key K\<rbrace>,
               Crypt (shrK B) \<lbrace>NB, Agent A, Agent B, Key K\<rbrace>\<rbrace>
            \<in> set evs;
-         evs \<in> otway |]
-      ==> K \<notin> range shrK \<and> (\<exists>i. NA = Nonce i) \<and> (\<exists>j. NB = Nonce j)"
+         evs \<in> otway\<rbrakk>
+      \<Longrightarrow> K \<notin> range shrK \<and> (\<exists>i. NA = Nonce i) \<and> (\<exists>j. NB = Nonce j)"
 apply (erule rev_mp)
 apply (erule otway.induct, auto)
 done
@@ -145,7 +145,7 @@ done
 (****
  The following is to prove theorems of the form
 
-  Key K \<in> analz (insert (Key KAB) (knows Spy evs)) ==>
+  Key K \<in> analz (insert (Key KAB) (knows Spy evs)) \<Longrightarrow>
   Key K \<in> analz (knows Spy evs)
 
  A more general formula must be proved inductively.
@@ -156,7 +156,7 @@ text\<open>Session keys are not used to encrypt other session keys\<close>
 
 text\<open>The equality makes the induction hypothesis easier to apply\<close>
 lemma analz_image_freshK [rule_format]:
- "evs \<in> otway ==>
+ "evs \<in> otway \<Longrightarrow>
    \<forall>K KK. KK \<subseteq> -(range shrK) \<longrightarrow>
           (Key K \<in> analz (Key`KK \<union> (knows Spy evs))) =
           (K \<in> KK | Key K \<in> analz (knows Spy evs))"
@@ -166,7 +166,7 @@ apply (drule_tac [7] OR4_analz_knows_Spy, analz_freshK, spy_analz, auto)
 done
 
 lemma analz_insert_freshK:
-  "[| evs \<in> otway;  KAB \<notin> range shrK |] ==>
+  "\<lbrakk>evs \<in> otway;  KAB \<notin> range shrK\<rbrakk> \<Longrightarrow>
       (Key K \<in> analz (insert (Key KAB) (knows Spy evs))) =
       (K = KAB | Key K \<in> analz (knows Spy evs))"
 by (simp only: analz_image_freshK analz_image_freshK_simps)
@@ -174,7 +174,7 @@ by (simp only: analz_image_freshK analz_image_freshK_simps)
 
 text\<open>The Key K uniquely identifies the Server's message.\<close>
 lemma unique_session_keys:
-     "[| Says Server B
+     "\<lbrakk>Says Server B
           \<lbrace>Crypt (shrK A) \<lbrace>NA, Agent A, Agent B, K\<rbrace>,
             Crypt (shrK B) \<lbrace>NB, Agent A, Agent B, K\<rbrace>\<rbrace>
          \<in> set evs;
@@ -182,8 +182,8 @@ lemma unique_session_keys:
           \<lbrace>Crypt (shrK A') \<lbrace>NA', Agent A', Agent B', K\<rbrace>,
             Crypt (shrK B') \<lbrace>NB', Agent A', Agent B', K\<rbrace>\<rbrace>
          \<in> set evs;
-        evs \<in> otway |]
-     ==> A=A' \<and> B=B' \<and> NA=NA' \<and> NB=NB'"
+        evs \<in> otway\<rbrakk>
+     \<Longrightarrow> A=A' \<and> B=B' \<and> NA=NA' \<and> NB=NB'"
 apply (erule rev_mp, erule rev_mp, erule otway.induct, simp_all)
 apply blast+  \<comment> \<open>OR3 and OR4\<close>
 done
@@ -193,8 +193,8 @@ subsection\<open>Authenticity properties relating to NA\<close>
 
 text\<open>If the encrypted message appears then it originated with the Server!\<close>
 lemma NA_Crypt_imp_Server_msg [rule_format]:
-    "[| A \<notin> bad;  A \<noteq> B;  evs \<in> otway |]
-     ==> Crypt (shrK A) \<lbrace>NA, Agent A, Agent B, Key K\<rbrace> \<in> parts (knows Spy evs)
+    "\<lbrakk>A \<notin> bad;  A \<noteq> B;  evs \<in> otway\<rbrakk>
+     \<Longrightarrow> Crypt (shrK A) \<lbrace>NA, Agent A, Agent B, Key K\<rbrace> \<in> parts (knows Spy evs)
        \<longrightarrow> (\<exists>NB. Says Server B
                     \<lbrace>Crypt (shrK A) \<lbrace>NA, Agent A, Agent B, Key K\<rbrace>,
                       Crypt (shrK B) \<lbrace>NB, Agent A, Agent B, Key K\<rbrace>\<rbrace>
@@ -208,9 +208,9 @@ done
 text\<open>Corollary: if A receives B's OR4 message then it originated with the
       Server. Freshness may be inferred from nonce NA.\<close>
 lemma A_trusts_OR4:
-     "[| Says B' A (Crypt (shrK A) \<lbrace>NA, Agent A, Agent B, Key K\<rbrace>) \<in> set evs;
-         A \<notin> bad;  A \<noteq> B;  evs \<in> otway |]
-      ==> \<exists>NB. Says Server B
+     "\<lbrakk>Says B' A (Crypt (shrK A) \<lbrace>NA, Agent A, Agent B, Key K\<rbrace>) \<in> set evs;
+         A \<notin> bad;  A \<noteq> B;  evs \<in> otway\<rbrakk>
+      \<Longrightarrow> \<exists>NB. Says Server B
                   \<lbrace>Crypt (shrK A) \<lbrace>NA, Agent A, Agent B, Key K\<rbrace>,
                     Crypt (shrK B) \<lbrace>NB, Agent A, Agent B, Key K\<rbrace>\<rbrace>
                  \<in> set evs"
@@ -221,8 +221,8 @@ text\<open>Crucial secrecy property: Spy does not see the keys sent in msg OR3
     Does not in itself guarantee security: an attack could violate
     the premises, e.g. by having \<^term>\<open>A=Spy\<close>\<close>
 lemma secrecy_lemma:
-     "[| A \<notin> bad;  B \<notin> bad;  evs \<in> otway |]
-      ==> Says Server B
+     "\<lbrakk>A \<notin> bad;  B \<notin> bad;  evs \<in> otway\<rbrakk>
+      \<Longrightarrow> Says Server B
            \<lbrace>Crypt (shrK A) \<lbrace>NA, Agent A, Agent B, Key K\<rbrace>,
              Crypt (shrK B) \<lbrace>NB, Agent A, Agent B, Key K\<rbrace>\<rbrace>
           \<in> set evs \<longrightarrow>
@@ -238,23 +238,23 @@ done
 
 
 lemma Spy_not_see_encrypted_key:
-     "[| Says Server B
+     "\<lbrakk>Says Server B
             \<lbrace>Crypt (shrK A) \<lbrace>NA, Agent A, Agent B, Key K\<rbrace>,
               Crypt (shrK B) \<lbrace>NB, Agent A, Agent B, Key K\<rbrace>\<rbrace>
            \<in> set evs;
          Notes Spy \<lbrace>NA, NB, Key K\<rbrace> \<notin> set evs;
-         A \<notin> bad;  B \<notin> bad;  evs \<in> otway |]
-      ==> Key K \<notin> analz (knows Spy evs)"
+         A \<notin> bad;  B \<notin> bad;  evs \<in> otway\<rbrakk>
+      \<Longrightarrow> Key K \<notin> analz (knows Spy evs)"
   by (metis secrecy_lemma)
 
 
 text\<open>A's guarantee.  The Oops premise quantifies over NB because A cannot know
   what it is.\<close>
 lemma A_gets_good_key:
-     "[| Says B' A (Crypt (shrK A) \<lbrace>NA, Agent A, Agent B, Key K\<rbrace>) \<in> set evs;
+     "\<lbrakk>Says B' A (Crypt (shrK A) \<lbrace>NA, Agent A, Agent B, Key K\<rbrace>) \<in> set evs;
          \<forall>NB. Notes Spy \<lbrace>NA, NB, Key K\<rbrace> \<notin> set evs;
-         A \<notin> bad;  B \<notin> bad;  A \<noteq> B;  evs \<in> otway |]
-      ==> Key K \<notin> analz (knows Spy evs)"
+         A \<notin> bad;  B \<notin> bad;  A \<noteq> B;  evs \<in> otway\<rbrakk>
+      \<Longrightarrow> Key K \<notin> analz (knows Spy evs)"
   by (metis A_trusts_OR4 secrecy_lemma)
 
 
@@ -263,8 +263,8 @@ subsection\<open>Authenticity properties relating to NB\<close>
 
 text\<open>If the encrypted message appears then it originated with the Server!\<close>
 lemma NB_Crypt_imp_Server_msg [rule_format]:
- "[| B \<notin> bad;  A \<noteq> B;  evs \<in> otway |]
-  ==> Crypt (shrK B) \<lbrace>NB, Agent A, Agent B, Key K\<rbrace> \<in> parts (knows Spy evs)
+ "\<lbrakk>B \<notin> bad;  A \<noteq> B;  evs \<in> otway\<rbrakk>
+  \<Longrightarrow> Crypt (shrK B) \<lbrace>NB, Agent A, Agent B, Key K\<rbrace> \<in> parts (knows Spy evs)
       \<longrightarrow> (\<exists>NA. Says Server B
                    \<lbrace>Crypt (shrK A) \<lbrace>NA, Agent A, Agent B, Key K\<rbrace>,
                      Crypt (shrK B) \<lbrace>NB, Agent A, Agent B, Key K\<rbrace>\<rbrace>
@@ -278,10 +278,10 @@ done
 text\<open>Guarantee for B: if it gets a well-formed certificate then the Server
   has sent the correct message in round 3.\<close>
 lemma B_trusts_OR3:
-     "[| Says S B \<lbrace>X, Crypt (shrK B) \<lbrace>NB, Agent A, Agent B, Key K\<rbrace>\<rbrace>
+     "\<lbrakk>Says S B \<lbrace>X, Crypt (shrK B) \<lbrace>NB, Agent A, Agent B, Key K\<rbrace>\<rbrace>
            \<in> set evs;
-         B \<notin> bad;  A \<noteq> B;  evs \<in> otway |]
-      ==> \<exists>NA. Says Server B
+         B \<notin> bad;  A \<noteq> B;  evs \<in> otway\<rbrakk>
+      \<Longrightarrow> \<exists>NA. Says Server B
                    \<lbrace>Crypt (shrK A) \<lbrace>NA, Agent A, Agent B, Key K\<rbrace>,
                      Crypt (shrK B) \<lbrace>NB, Agent A, Agent B, Key K\<rbrace>\<rbrace>
                    \<in> set evs"
@@ -291,11 +291,11 @@ by (blast intro!: NB_Crypt_imp_Server_msg)
 text\<open>The obvious combination of \<open>B_trusts_OR3\<close> with 
       \<open>Spy_not_see_encrypted_key\<close>\<close>
 lemma B_gets_good_key:
-     "[| Gets B \<lbrace>X, Crypt (shrK B) \<lbrace>NB, Agent A, Agent B, Key K\<rbrace>\<rbrace>
+     "\<lbrakk>Gets B \<lbrace>X, Crypt (shrK B) \<lbrace>NB, Agent A, Agent B, Key K\<rbrace>\<rbrace>
           \<in> set evs;
          \<forall>NA. Notes Spy \<lbrace>NA, NB, Key K\<rbrace> \<notin> set evs;
-         A \<notin> bad;  B \<notin> bad;  A \<noteq> B;  evs \<in> otway |]
-      ==> Key K \<notin> analz (knows Spy evs)"
+         A \<notin> bad;  B \<notin> bad;  A \<noteq> B;  evs \<in> otway\<rbrakk>
+      \<Longrightarrow> Key K \<notin> analz (knows Spy evs)"
 by (blast dest: B_trusts_OR3 Spy_not_see_encrypted_key)
 
 end
